theories/case_studies/dle/deep_locality_concrete.v
@@ -14,74 +14,67 @@ Local Notation "'A' z" :=
 Local Notation "'OT' z" :=
   (@finz.FinZ ONum z%Z eq_refl eq_refl) (at level 10).
 
-Definition dle_main_pcc_begin : Addr := A 9.
+Definition dle_main_pcc_b : Addr := A 9.
 Definition dle_main_code_start : Addr := A 12.
-Definition dle_main_pcc_end : Addr := A 67.
-Definition dle_main_data_begin : Addr := A 74.
-Definition dle_main_data_end : Addr := A 76.
+Definition dle_main_pcc_e : Addr := A 67.
+Definition dle_main_data_b : Addr := A 74.
+Definition dle_main_data_e : Addr := A 76.
 Definition dle_main_exports_pcc : Addr := A 77.
 Definition dle_main_exports_cgp : Addr := A 78.
-Definition dle_main_exports_entries_begin : Addr := A 79.
-Definition dle_main_exports_entries_end : Addr := A 79.
+Definition dle_main_exports_entries_b : Addr := A 79.
+Definition dle_main_exports_entries_e : Addr := A 79.
 
-Definition dle_C_pcc_begin : Addr := A 67.
+Definition dle_C_pcc_b : Addr := A 67.
 Definition dle_C_code_start : Addr := A 68.
-Definition dle_C_pcc_end : Addr := A 74.
-Definition dle_C_data_begin : Addr := A 76.
-Definition dle_C_data_end : Addr := A 77.
+Definition dle_C_pcc_e : Addr := A 74.
+Definition dle_C_data_b : Addr := A 76.
+Definition dle_C_data_e : Addr := A 77.
 Definition dle_C_exports_pcc : Addr := A 79.
 Definition dle_C_exports_cgp : Addr := A 80.
-Definition dle_C_exports_entries_begin : Addr := A 81.
-Definition dle_C_exports_entries_end : Addr := A 82.
+Definition dle_C_exports_entries_b : Addr := A 81.
+Definition dle_C_exports_entries_e : Addr := A 82.
 
-Definition dle_assert_begin : Addr := A 82.
+Definition dle_assert_b : Addr := A 82.
 Definition dle_assert_cap : Addr := A 94.
-Definition dle_assert_end : Addr := A 95.
+Definition dle_assert_e : Addr := A 95.
 Definition dle_assert_flag : Addr := A 95.
 
-Definition dle_switcher_begin : Addr := A 96.
+Definition dle_switcher_b : Addr := A 96.
 Definition dle_switcher_call : Addr := A 97.
 Definition dle_switcher_return : Addr := A 185.
-Definition dle_switcher_end : Addr := A 247.
+Definition dle_switcher_e : Addr := A 247.
 Definition dle_switcher_sealing_type : OType := OT 9.
 
-Definition dle_trusted_stack_begin : Addr := A 4096.
-Definition dle_trusted_stack_end : Addr := A 4196.
-Definition dle_stack_begin : Addr := A 1024.
-Definition dle_stack_end : Addr := A 1124.
+Definition dle_trusted_stack_b : Addr := A 4096.
+Definition dle_trusted_stack_e : Addr := A 4196.
+Definition dle_stack_b : Addr := A 1024.
+Definition dle_stack_e : Addr := A 1124.
 
 Ltac unfold_dle_addresses :=
-  unfold dle_main_pcc_begin, dle_main_code_start, dle_main_pcc_end,
-    dle_main_data_begin, dle_main_data_end, dle_main_exports_pcc,
-    dle_main_exports_cgp, dle_main_exports_entries_begin,
-    dle_main_exports_entries_end, dle_C_pcc_begin, dle_C_code_start,
-    dle_C_pcc_end, dle_C_data_begin, dle_C_data_end, dle_C_exports_pcc,
-    dle_C_exports_cgp, dle_C_exports_entries_begin,
-    dle_C_exports_entries_end, dle_assert_begin, dle_assert_cap,
-    dle_assert_end, dle_assert_flag, dle_switcher_begin, dle_switcher_call,
-    dle_switcher_return, dle_switcher_end, dle_switcher_sealing_type,
-    dle_trusted_stack_begin, dle_trusted_stack_end, dle_stack_begin,
-    dle_stack_end.
+  unfold dle_main_pcc_b, dle_main_code_start, dle_main_pcc_e,
+    dle_main_data_b, dle_main_data_e, dle_main_exports_pcc,
+    dle_main_exports_cgp, dle_main_exports_entries_b,
+    dle_main_exports_entries_e, dle_C_pcc_b, dle_C_code_start,
+    dle_C_pcc_e, dle_C_data_b, dle_C_data_e, dle_C_exports_pcc,
+    dle_C_exports_cgp, dle_C_exports_entries_b,
+    dle_C_exports_entries_e, dle_assert_b, dle_assert_cap,
+    dle_assert_e, dle_assert_flag, dle_switcher_b, dle_switcher_call,
+    dle_switcher_return, dle_switcher_e, dle_switcher_sealing_type,
+    dle_trusted_stack_b, dle_trusted_stack_e, dle_stack_b,
+    dle_stack_e.
 
 Ltac unfold_dle_addresses_in H :=
-  unfold dle_main_pcc_begin, dle_main_code_start, dle_main_pcc_end,
-    dle_main_data_begin, dle_main_data_end, dle_main_exports_pcc,
-    dle_main_exports_cgp, dle_main_exports_entries_begin,
-    dle_main_exports_entries_end, dle_C_pcc_begin, dle_C_code_start,
-    dle_C_pcc_end, dle_C_data_begin, dle_C_data_end, dle_C_exports_pcc,
-    dle_C_exports_cgp, dle_C_exports_entries_begin,
-    dle_C_exports_entries_end, dle_assert_begin, dle_assert_cap,
-    dle_assert_end, dle_assert_flag, dle_switcher_begin, dle_switcher_call,
-    dle_switcher_return, dle_switcher_end, dle_switcher_sealing_type,
-    dle_trusted_stack_begin, dle_trusted_stack_end, dle_stack_begin,
-    dle_stack_end in H.
-
-Definition dle_C_nested_read : instr.
-Proof.
-  constructor 5.
-  - exact ct0.
-  - exact ca0.
-Defined.
+  unfold dle_main_pcc_b, dle_main_code_start, dle_main_pcc_e,
+    dle_main_data_b, dle_main_data_e, dle_main_exports_pcc,
+    dle_main_exports_cgp, dle_main_exports_entries_b,
+    dle_main_exports_entries_e, dle_C_pcc_b, dle_C_code_start,
+    dle_C_pcc_e, dle_C_data_b, dle_C_data_e, dle_C_exports_pcc,
+    dle_C_exports_cgp, dle_C_exports_entries_b,
+    dle_C_exports_entries_e, dle_assert_b, dle_assert_cap,
+    dle_assert_e, dle_assert_flag, dle_switcher_b, dle_switcher_call,
+    dle_switcher_return, dle_switcher_e, dle_switcher_sealing_type,
+    dle_trusted_stack_b, dle_trusted_stack_e, dle_stack_b,
+    dle_stack_e in H.
 
 (** The concrete adversary examines the argument passed in [ca0]. If it is a
     capability, the adversary follows it to the nested capability and attempts
@@ -92,7 +85,7 @@ Definition dle_C_code : list Word :=
     GetWType ct0 ca0;
     Sub ct0 ct0 (encodeWordType wt_cap);
     Jnz 3%Z ct0;
-    dle_C_nested_read;
+    Load ct0 ca0;
     Store ct0 7%Z;
     Jalr cnull cra
   ].
@@ -100,7 +93,7 @@ Definition dle_C_code : list Word :=
 Definition dle_C_data : list Word := [WInt 0].
 
 Definition dle_C_imports : list Word :=
-  [WSentry XSRW_ Local dle_switcher_begin dle_switcher_end dle_switcher_call].
+  [WSentry XSRW_ Local dle_switcher_b dle_switcher_e dle_switcher_call].
 
 Definition dle_C_exports : list Word :=
   [WInt (encode_entry_point 1 1)].
@@ -108,12 +101,12 @@ Definition dle_C_exports : list Word :=
 Program Definition dle_concrete_cmptSwitcher : cmptSwitcher.
 Proof.
   refine (@mkCmptSwitcher machine_parameters_instance
-    dle_switcher_begin dle_switcher_end
+    dle_switcher_b dle_switcher_e
     dle_switcher_call dle_switcher_return dle_switcher_sealing_type
-    dle_trusted_stack_begin dle_trusted_stack_end
+    dle_trusted_stack_b dle_trusted_stack_e
     _ _ _ _
     (replicate 100 (WInt 0)) _ eq_refl
-    dle_stack_begin dle_stack_end (replicate 100 (WInt 0)) _ _).
+    dle_stack_b dle_stack_e (replicate 100 (WInt 0)) _ _).
   - vm_compute; solve_addr.
   - vm_compute; solve_addr.
   - vm_compute; solve_addr.
@@ -129,7 +122,7 @@ Defined.
 Program Definition dle_concrete_cmptAssert : cmptAssert.
 Proof.
   refine (@mkCmptAssert machine_parameters_instance
-    dle_assert_begin dle_assert_end dle_assert_cap dle_assert_flag _ _ _ _).
+    dle_assert_b dle_assert_e dle_assert_cap dle_assert_flag _ _ _ _).
   - vm_compute; solve_addr.
   - vm_compute; solve_addr.
   - vm_compute; solve_addr.
@@ -151,8 +144,8 @@ Proof.
 Defined.
 
 Definition dle_C_f : Sealable :=
-  SCap RO Global dle_C_exports_pcc dle_C_exports_entries_end
-    dle_C_exports_entries_begin.
+  SCap RO Global dle_C_exports_pcc dle_C_exports_entries_e
+    dle_C_exports_entries_b.
 
 Definition dle_main_imports_concrete : list Word :=
   dle_main_imports dle_C_f.
@@ -160,10 +153,10 @@ Definition dle_main_imports_concrete : list Word :=
 Program Definition dle_concrete_main_cmpt : cmpt.
 Proof.
   refine (@mkCmpt
-    dle_main_pcc_begin dle_main_code_start dle_main_pcc_end
-    dle_main_data_begin dle_main_data_end
+    dle_main_pcc_b dle_main_code_start dle_main_pcc_e
+    dle_main_data_b dle_main_data_e
     dle_main_exports_pcc dle_main_exports_cgp
-    dle_main_exports_entries_begin dle_main_exports_entries_end
+    dle_main_exports_entries_b dle_main_exports_entries_e
     dle_main_imports_concrete dle_main_code dle_main_data []
     _ _ _ _ _ _ _).
   - vm_compute; solve_addr.
@@ -178,10 +171,10 @@ Defined.
 Program Definition dle_concrete_C_cmpt : cmpt.
 Proof.
   refine (@mkCmpt
-    dle_C_pcc_begin dle_C_code_start dle_C_pcc_end
-    dle_C_data_begin dle_C_data_end
+    dle_C_pcc_b dle_C_code_start dle_C_pcc_e
+    dle_C_data_b dle_C_data_e
     dle_C_exports_pcc dle_C_exports_cgp
-    dle_C_exports_entries_begin dle_C_exports_entries_end
+    dle_C_exports_entries_b dle_C_exports_entries_e
     dle_C_imports dle_C_code dle_C_data dle_C_exports
     _ _ _ _ _ _ _).
   - vm_compute; solve_addr.
@@ -225,15 +218,15 @@ Proof.
 Defined.
 
 Definition dle_initial_registers : Reg :=
-  <[PC := WCap RX Global dle_main_pcc_begin dle_main_pcc_end dle_main_code_start]>
-  (<[cgp := WCap RW Global dle_main_data_begin dle_main_data_end
-      dle_main_data_begin]>
-  (<[csp := WCap RWL Local dle_stack_begin dle_stack_end dle_stack_begin]>
+  <[PC := WCap RX Global dle_main_pcc_b dle_main_pcc_e dle_main_code_start]>
+  (<[cgp := WCap RW Global dle_main_data_b dle_main_data_e
+      dle_main_data_b]>
+  (<[csp := WCap RWL Local dle_stack_b dle_stack_e dle_stack_b]>
     (gset_to_gmap (WInt 0) all_registers_s))).
 
 Definition dle_initial_sregisters : SReg :=
-  <[MTDC := WCap RWL Local dle_trusted_stack_begin dle_trusted_stack_end
-      dle_trusted_stack_begin]> ∅.
+  <[MTDC := WCap RWL Local dle_trusted_stack_b dle_trusted_stack_e
+      dle_trusted_stack_b]> ∅.
 
 Definition dle_initial_memory : Mem := mk_initial_memory.
 
@@ -271,7 +264,7 @@ Proof.
   - apply Forall_replicate; done.
 Qed.
 
-Theorem dle_concrete_adequacy reg' sreg' mem' es :
+Lemma dle_concrete_adequacy reg' sreg' mem' es :
   rtc erased_step
     ([Seq (Instr Executable)],
       (dle_initial_registers, dle_initial_sregisters, dle_initial_memory))
