theories/case_studies/lse_downward/lse_concrete.v
@@ -12,72 +12,65 @@ Local Notation "'A' z" :=
 Local Notation "'OT' z" :=
   (@finz.FinZ ONum z%Z eq_refl eq_refl) (at level 10).
 
-Definition lse_main_pcc_begin : Addr := A 9.
+Definition lse_main_pcc_b : Addr := A 9.
 Definition lse_main_code_start : Addr := A 12.
-Definition lse_main_pcc_end : Addr := A 56.
-Definition lse_C_pcc_begin : Addr := A 56.
+Definition lse_main_pcc_e : Addr := A 56.
+Definition lse_C_pcc_b : Addr := A 56.
 Definition lse_C_code_start : Addr := A 58.
-Definition lse_C_pcc_end : Addr := A 99.
-Definition lse_main_data_begin : Addr := A 99.
-Definition lse_main_data_end : Addr := A 100.
-Definition lse_C_data_begin : Addr := A 100.
-Definition lse_C_data_end : Addr := A 101.
+Definition lse_C_pcc_e : Addr := A 99.
+Definition lse_main_data_b : Addr := A 99.
+Definition lse_main_data_e : Addr := A 100.
+Definition lse_C_data_b : Addr := A 100.
+Definition lse_C_data_e : Addr := A 101.
 Definition lse_main_exports_pcc : Addr := A 101.
 Definition lse_main_exports_cgp : Addr := A 102.
-Definition lse_main_exports_entries_begin : Addr := A 103.
-Definition lse_main_exports_entries_end : Addr := A 104.
+Definition lse_main_exports_entries_b : Addr := A 103.
+Definition lse_main_exports_entries_e : Addr := A 104.
 Definition lse_C_exports_pcc : Addr := A 104.
 Definition lse_C_exports_cgp : Addr := A 105.
-Definition lse_C_exports_entries_begin : Addr := A 106.
-Definition lse_C_exports_entries_end : Addr := A 107.
-Definition lse_assert_begin : Addr := A 107.
+Definition lse_C_exports_entries_b : Addr := A 106.
+Definition lse_C_exports_entries_e : Addr := A 107.
+Definition lse_assert_b : Addr := A 107.
 Definition lse_assert_cap : Addr := A 119.
-Definition lse_assert_end : Addr := A 120.
+Definition lse_assert_e : Addr := A 120.
 Definition lse_assert_flag : Addr := A 120.
-Definition lse_switcher_begin : Addr := A 121.
+Definition lse_switcher_b : Addr := A 121.
 Definition lse_switcher_call : Addr := A 122.
 Definition lse_switcher_return : Addr := A 210.
-Definition lse_switcher_end : Addr := A 272.
+Definition lse_switcher_e : Addr := A 272.
 Definition lse_switcher_sealing_type : OType := OT 9.
-Definition lse_trusted_stack_begin : Addr := A 4096.
-Definition lse_trusted_stack_end : Addr := A 4196.
-Definition lse_stack_begin : Addr := A 1024.
-Definition lse_stack_end : Addr := A 1124.
+Definition lse_trusted_stack_b : Addr := A 4096.
+Definition lse_trusted_stack_e : Addr := A 4196.
+Definition lse_stack_b : Addr := A 1024.
+Definition lse_stack_e : Addr := A 1124.
 
 Ltac unfold_lse_addresses :=
-  unfold lse_main_pcc_begin, lse_main_code_start, lse_main_pcc_end,
-    lse_C_pcc_begin, lse_C_code_start, lse_C_pcc_end,
-    lse_main_data_begin, lse_main_data_end, lse_C_data_begin, lse_C_data_end,
+  unfold lse_main_pcc_b, lse_main_code_start, lse_main_pcc_e,
+    lse_C_pcc_b, lse_C_code_start, lse_C_pcc_e,
+    lse_main_data_b, lse_main_data_e, lse_C_data_b, lse_C_data_e,
     lse_main_exports_pcc, lse_main_exports_cgp,
-    lse_main_exports_entries_begin, lse_main_exports_entries_end,
+    lse_main_exports_entries_b, lse_main_exports_entries_e,
     lse_C_exports_pcc, lse_C_exports_cgp,
-    lse_C_exports_entries_begin, lse_C_exports_entries_end,
-    lse_assert_begin, lse_assert_cap, lse_assert_end, lse_assert_flag,
-    lse_switcher_begin, lse_switcher_call, lse_switcher_return,
-    lse_switcher_end, lse_switcher_sealing_type,
-    lse_trusted_stack_begin, lse_trusted_stack_end,
-    lse_stack_begin, lse_stack_end.
+    lse_C_exports_entries_b, lse_C_exports_entries_e,
+    lse_assert_b, lse_assert_cap, lse_assert_e, lse_assert_flag,
+    lse_switcher_b, lse_switcher_call, lse_switcher_return,
+    lse_switcher_e, lse_switcher_sealing_type,
+    lse_trusted_stack_b, lse_trusted_stack_e,
+    lse_stack_b, lse_stack_e.
 
 Ltac unfold_lse_addresses_in H :=
-  unfold lse_main_pcc_begin, lse_main_code_start, lse_main_pcc_end,
-    lse_C_pcc_begin, lse_C_code_start, lse_C_pcc_end,
-    lse_main_data_begin, lse_main_data_end, lse_C_data_begin, lse_C_data_end,
+  unfold lse_main_pcc_b, lse_main_code_start, lse_main_pcc_e,
+    lse_C_pcc_b, lse_C_code_start, lse_C_pcc_e,
+    lse_main_data_b, lse_main_data_e, lse_C_data_b, lse_C_data_e,
     lse_main_exports_pcc, lse_main_exports_cgp,
-    lse_main_exports_entries_begin, lse_main_exports_entries_end,
+    lse_main_exports_entries_b, lse_main_exports_entries_e,
     lse_C_exports_pcc, lse_C_exports_cgp,
-    lse_C_exports_entries_begin, lse_C_exports_entries_end,
-    lse_assert_begin, lse_assert_cap, lse_assert_end, lse_assert_flag,
-    lse_switcher_begin, lse_switcher_call, lse_switcher_return,
-    lse_switcher_end, lse_switcher_sealing_type,
-    lse_trusted_stack_begin, lse_trusted_stack_end,
-    lse_stack_begin, lse_stack_end in H.
-
-Definition lse_C_load (dst src : RegName) : instr.
-Proof.
-  constructor 5.
-  - exact dst.
-  - exact src.
-Defined.
+    lse_C_exports_entries_b, lse_C_exports_entries_e,
+    lse_assert_b, lse_assert_cap, lse_assert_e, lse_assert_flag,
+    lse_switcher_b, lse_switcher_call, lse_switcher_return,
+    lse_switcher_e, lse_switcher_sealing_type,
+    lse_trusted_stack_b, lse_trusted_stack_e,
+    lse_stack_b, lse_stack_e in H.
 
 (** The concrete adversary saves its outer return capability, fetches the
     switcher and the exported main function, and calls the function twice. It
@@ -85,22 +78,50 @@ Defined.
     restores its return capability and returns to the caller. *)
 Definition lse_C_code : list Word :=
   encodeInstrsW [
-    Store csp cra; Lea csp 1%Z;
+    Store csp cra;
+    Lea csp 1%Z;
 
-    Mov ct0 PC; GetB cs0 ct0; GetA cs1 ct0; Sub cs0 cs0 cs1;
-    Lea ct0 cs0; Lea ct0 0%Z; lse_C_load ct0 ct0; Mov cs0 0%Z;
-    Mov ct1 PC; GetB cs0 ct1; GetA cs1 ct1; Sub cs0 cs0 cs1;
-    Lea ct1 cs0; Lea ct1 1%Z; lse_C_load ct1 ct1; Mov cs0 0%Z;
+    Mov ct0 PC;
+    GetB cs0 ct0;
+    GetA cs1 ct0;
+    Sub cs0 cs0 cs1;
+    Lea ct0 cs0;
+    Lea ct0 0%Z;
+    Load ct0 ct0;
+    Mov cs0 0%Z;
+    Mov ct1 PC;
+    GetB cs0 ct1;
+    GetA cs1 ct1;
+    Sub cs0 cs0 cs1;
+    Lea ct1 cs0;
+    Lea ct1 1%Z;
+    Load ct1 ct1;
+    Mov cs0 0%Z;
     Jalr cra ct0;
 
-    Mov ct0 PC; GetB cs0 ct0; GetA cs1 ct0; Sub cs0 cs0 cs1;
-    Lea ct0 cs0; Lea ct0 0%Z; lse_C_load ct0 ct0; Mov cs0 0%Z;
-    Mov ct1 PC; GetB cs0 ct1; GetA cs1 ct1; Sub cs0 cs0 cs1;
-    Lea ct1 cs0; Lea ct1 1%Z; lse_C_load ct1 ct1; Mov cs0 0%Z;
+    Mov ct0 PC;
+    GetB cs0 ct0;
+    GetA cs1 ct0;
+    Sub cs0 cs0 cs1;
+    Lea ct0 cs0;
+    Lea ct0 0%Z;
+    Load ct0 ct0;
+    Mov cs0 0%Z;
+    Mov ct1 PC;
+    GetB cs0 ct1;
+    GetA cs1 ct1;
+    Sub cs0 cs0 cs1;
+    Lea ct1 cs0;
+    Lea ct1 1%Z;
+    Load ct1 ct1;
+    Mov cs0 0%Z;
     Jalr cra ct0;
 
-    Lea csp (-1)%Z; lse_C_load cra csp;
-    Mov ca0 0%Z; Mov ca1 0%Z; Jalr cnull cra
+    Lea csp (-1)%Z;
+    Load cra csp;
+    Mov ca0 0%Z;
+    Mov ca1 0%Z;
+    Jalr cnull cra
   ].
 
 Definition lse_C_data : list Word := [WInt 0].
@@ -108,12 +129,12 @@ Definition lse_C_data : list Word := [WInt 0].
 Program Definition lse_concrete_cmptSwitcher : cmptSwitcher.
 Proof.
   refine (@mkCmptSwitcher machine_parameters_instance
-    lse_switcher_begin lse_switcher_end
+    lse_switcher_b lse_switcher_e
     lse_switcher_call lse_switcher_return lse_switcher_sealing_type
-    lse_trusted_stack_begin lse_trusted_stack_end
+    lse_trusted_stack_b lse_trusted_stack_e
     _ _ _ _
     (replicate 100 (WInt 0)) _ eq_refl
-    lse_stack_begin lse_stack_end (replicate 100 (WInt 0)) _ _).
+    lse_stack_b lse_stack_e (replicate 100 (WInt 0)) _ _).
   - vm_compute; solve_addr.
   - vm_compute; solve_addr.
   - vm_compute; solve_addr.
@@ -129,7 +150,7 @@ Defined.
 Program Definition lse_concrete_cmptAssert : cmptAssert.
 Proof.
   refine (@mkCmptAssert machine_parameters_instance
-    lse_assert_begin lse_assert_end lse_assert_cap lse_assert_flag _ _ _ _).
+    lse_assert_b lse_assert_e lse_assert_cap lse_assert_flag _ _ _ _).
   - vm_compute; solve_addr.
   - vm_compute; solve_addr.
   - vm_compute; solve_addr.
@@ -151,15 +172,15 @@ Proof.
 Defined.
 
 Definition lse_C_f : Sealable :=
-  SCap RO Global lse_C_exports_pcc lse_C_exports_entries_end
-    lse_C_exports_entries_begin.
+  SCap RO Global lse_C_exports_pcc lse_C_exports_entries_e
+    lse_C_exports_entries_b.
 
 Definition lse_main_imports_concrete : list Word := lse_main_imports lse_C_f.
 
 Definition lse_C_imports : list Word :=
-  [ WSentry XSRW_ Local lse_switcher_begin lse_switcher_end lse_switcher_call
+  [ WSentry XSRW_ Local lse_switcher_b lse_switcher_e lse_switcher_call
   ; WSealed lse_switcher_sealing_type
-      (lse_entry_f_sb lse_main_exports_pcc lse_main_exports_entries_end)
+      (lse_entry_f_sb lse_main_exports_pcc lse_main_exports_entries_e)
   ].
 
 Definition lse_C_exports : list Word := [WInt (encode_entry_point 0 2)].
@@ -167,10 +188,10 @@ Definition lse_C_exports : list Word := [WInt (encode_entry_point 0 2)].
 Program Definition lse_concrete_main_cmpt : cmpt.
 Proof.
   refine (@mkCmpt
-    lse_main_pcc_begin lse_main_code_start lse_main_pcc_end
-    lse_main_data_begin lse_main_data_end
+    lse_main_pcc_b lse_main_code_start lse_main_pcc_e
+    lse_main_data_b lse_main_data_e
     lse_main_exports_pcc lse_main_exports_cgp
-    lse_main_exports_entries_begin lse_main_exports_entries_end
+    lse_main_exports_entries_b lse_main_exports_entries_e
     lse_main_imports_concrete lse_main_code lse_main_data lse_export_table_entries
     _ _ _ _ _ _ _).
   - vm_compute; solve_addr.
@@ -185,10 +206,10 @@ Defined.
 Program Definition lse_concrete_C_cmpt : cmpt.
 Proof.
   refine (@mkCmpt
-    lse_C_pcc_begin lse_C_code_start lse_C_pcc_end
-    lse_C_data_begin lse_C_data_end
+    lse_C_pcc_b lse_C_code_start lse_C_pcc_e
+    lse_C_data_b lse_C_data_e
     lse_C_exports_pcc lse_C_exports_cgp
-    lse_C_exports_entries_begin lse_C_exports_entries_end
+    lse_C_exports_entries_b lse_C_exports_entries_e
     lse_C_imports lse_C_code lse_C_data lse_C_exports
     _ _ _ _ _ _ _).
   - vm_compute; solve_addr.
@@ -232,15 +253,15 @@ Proof.
 Defined.
 
 Definition lse_initial_registers : Reg :=
-  <[PC := WCap RX Global lse_main_pcc_begin lse_main_pcc_end lse_main_code_start]>
-  (<[cgp := WCap RW Global lse_main_data_begin lse_main_data_end
-      lse_main_data_begin]>
-  (<[csp := WCap RWL Local lse_stack_begin lse_stack_end lse_stack_begin]>
+  <[PC := WCap RX Global lse_main_pcc_b lse_main_pcc_e lse_main_code_start]>
+  (<[cgp := WCap RW Global lse_main_data_b lse_main_data_e
+      lse_main_data_b]>
+  (<[csp := WCap RWL Local lse_stack_b lse_stack_e lse_stack_b]>
     (gset_to_gmap (WInt 0) all_registers_s))).
 
 Definition lse_initial_sregisters : SReg :=
-  <[MTDC := WCap RWL Local lse_trusted_stack_begin lse_trusted_stack_end
-      lse_trusted_stack_begin]> ∅.
+  <[MTDC := WCap RWL Local lse_trusted_stack_b lse_trusted_stack_e
+      lse_trusted_stack_b]> ∅.
 
 Definition lse_initial_memory : Mem := mk_initial_memory.
 
@@ -276,7 +297,7 @@ Proof.
   - apply Forall_replicate; done.
 Qed.
 
-Theorem lse_concrete_adequacy reg' sreg' mem' es :
+Lemma lse_concrete_adequacy reg' sreg' mem' es :
   rtc erased_step
     ([Seq (Instr Executable)],
       (lse_initial_registers, lse_initial_sregisters, lse_initial_memory))
