theories/case_studies/stack_object/stack_object_concrete.v
@@ -12,72 +12,65 @@ Local Notation "'A' z" :=
 Local Notation "'OT' z" :=
   (@finz.FinZ ONum z%Z eq_refl eq_refl) (at level 10).
 
-Definition so_main_pcc_begin : Addr := A 9.
+Definition so_main_pcc_b : Addr := A 9.
 Definition so_main_code_start : Addr := A 12.
-Definition so_main_pcc_end : Addr := A 160.
-Definition so_C_pcc_begin : Addr := A 160.
+Definition so_main_pcc_e : Addr := A 160.
+Definition so_C_pcc_b : Addr := A 160.
 Definition so_C_code_start : Addr := A 163.
-Definition so_C_pcc_end : Addr := A 204.
-Definition so_main_data_begin : Addr := A 204.
-Definition so_main_data_end : Addr := A 204.
-Definition so_C_data_begin : Addr := A 204.
-Definition so_C_data_end : Addr := A 205.
+Definition so_C_pcc_e : Addr := A 204.
+Definition so_main_data_b : Addr := A 204.
+Definition so_main_data_e : Addr := A 204.
+Definition so_C_data_b : Addr := A 204.
+Definition so_C_data_e : Addr := A 205.
 Definition so_main_exports_pcc : Addr := A 205.
 Definition so_main_exports_cgp : Addr := A 206.
-Definition so_main_exports_entries_begin : Addr := A 207.
-Definition so_main_exports_entries_end : Addr := A 208.
+Definition so_main_exports_entries_b : Addr := A 207.
+Definition so_main_exports_entries_e : Addr := A 208.
 Definition so_C_exports_pcc : Addr := A 208.
 Definition so_C_exports_cgp : Addr := A 209.
-Definition so_C_exports_entries_begin : Addr := A 210.
-Definition so_C_exports_entries_end : Addr := A 212.
-Definition so_assert_begin : Addr := A 212.
+Definition so_C_exports_entries_b : Addr := A 210.
+Definition so_C_exports_entries_e : Addr := A 212.
+Definition so_assert_b : Addr := A 212.
 Definition so_assert_cap : Addr := A 224.
-Definition so_assert_end : Addr := A 225.
+Definition so_assert_e : Addr := A 225.
 Definition so_assert_flag : Addr := A 225.
-Definition so_switcher_begin : Addr := A 226.
+Definition so_switcher_b : Addr := A 226.
 Definition so_switcher_call : Addr := A 227.
 Definition so_switcher_return : Addr := A 315.
-Definition so_switcher_end : Addr := A 377.
+Definition so_switcher_e : Addr := A 377.
 Definition so_switcher_sealing_type : OType := OT 9.
-Definition so_trusted_stack_begin : Addr := A 4096.
-Definition so_trusted_stack_end : Addr := A 4196.
-Definition so_stack_begin : Addr := A 1024.
-Definition so_stack_end : Addr := A 1124.
+Definition so_trusted_stack_b : Addr := A 4096.
+Definition so_trusted_stack_e : Addr := A 4196.
+Definition so_stack_b : Addr := A 1024.
+Definition so_stack_e : Addr := A 1124.
 
 Ltac unfold_so_addresses :=
-  unfold so_main_pcc_begin, so_main_code_start, so_main_pcc_end,
-    so_C_pcc_begin, so_C_code_start, so_C_pcc_end,
-    so_main_data_begin, so_main_data_end, so_C_data_begin, so_C_data_end,
+  unfold so_main_pcc_b, so_main_code_start, so_main_pcc_e,
+    so_C_pcc_b, so_C_code_start, so_C_pcc_e,
+    so_main_data_b, so_main_data_e, so_C_data_b, so_C_data_e,
     so_main_exports_pcc, so_main_exports_cgp,
-    so_main_exports_entries_begin, so_main_exports_entries_end,
+    so_main_exports_entries_b, so_main_exports_entries_e,
     so_C_exports_pcc, so_C_exports_cgp,
-    so_C_exports_entries_begin, so_C_exports_entries_end,
-    so_assert_begin, so_assert_cap, so_assert_end, so_assert_flag,
-    so_switcher_begin, so_switcher_call, so_switcher_return,
-    so_switcher_end, so_switcher_sealing_type,
-    so_trusted_stack_begin, so_trusted_stack_end,
-    so_stack_begin, so_stack_end.
+    so_C_exports_entries_b, so_C_exports_entries_e,
+    so_assert_b, so_assert_cap, so_assert_e, so_assert_flag,
+    so_switcher_b, so_switcher_call, so_switcher_return,
+    so_switcher_e, so_switcher_sealing_type,
+    so_trusted_stack_b, so_trusted_stack_e,
+    so_stack_b, so_stack_e.
 
 Ltac unfold_so_addresses_in H :=
-  unfold so_main_pcc_begin, so_main_code_start, so_main_pcc_end,
-    so_C_pcc_begin, so_C_code_start, so_C_pcc_end,
-    so_main_data_begin, so_main_data_end, so_C_data_begin, so_C_data_end,
+  unfold so_main_pcc_b, so_main_code_start, so_main_pcc_e,
+    so_C_pcc_b, so_C_code_start, so_C_pcc_e,
+    so_main_data_b, so_main_data_e, so_C_data_b, so_C_data_e,
     so_main_exports_pcc, so_main_exports_cgp,
-    so_main_exports_entries_begin, so_main_exports_entries_end,
+    so_main_exports_entries_b, so_main_exports_entries_e,
     so_C_exports_pcc, so_C_exports_cgp,
-    so_C_exports_entries_begin, so_C_exports_entries_end,
-    so_assert_begin, so_assert_cap, so_assert_end, so_assert_flag,
-    so_switcher_begin, so_switcher_call, so_switcher_return,
-    so_switcher_end, so_switcher_sealing_type,
-    so_trusted_stack_begin, so_trusted_stack_end,
-    so_stack_begin, so_stack_end in H.
-
-Definition so_C_load (dst src : RegName) : instr.
-Proof.
-  constructor 5.
-  - exact dst.
-  - exact src.
-Defined.
+    so_C_exports_entries_b, so_C_exports_entries_e,
+    so_assert_b, so_assert_cap, so_assert_e, so_assert_flag,
+    so_switcher_b, so_switcher_call, so_switcher_return,
+    so_switcher_e, so_switcher_sealing_type,
+    so_trusted_stack_b, so_trusted_stack_e,
+    so_stack_b, so_stack_e in H.
 
 (** The concrete adversary allocates and initializes a one-word public object
     on its stack, then calls the main function with that object and callback
@@ -87,19 +80,47 @@ Defined.
     before returning to the main program. *)
 Definition so_C_code : list Word :=
   encodeInstrsW [
-    Store csp cra; Lea csp 1%Z;
-    Mov ca0 csp; GetA cs0 ca0; machine_instructions.Add cs1 cs0 1%Z;
-    Subseg ca0 cs0 cs1; Store ca0 0%Z; Lea csp 1%Z;
-    Mov ctp PC; GetB cs0 ctp; GetA cs1 ctp; Sub cs0 cs0 cs1; Lea ctp cs0;
-    Mov ct0 ctp; Lea ct0 0%Z; so_C_load ct0 ct0;
-    Mov ct1 ctp; Lea ct1 1%Z; so_C_load ct1 ct1;
-    Mov ca1 ctp; Lea ca1 2%Z; so_C_load ca1 ca1;
-    Mov cs0 0%Z; Mov cs1 0%Z;
-    Mov cs0 cra; Mov cs1 ct1; Jalr cra ct0;
-    Lea csp (-1)%Z; Lea csp (-1)%Z; so_C_load cra csp;
-    Mov ca0 0%Z; Mov ca1 0%Z; Mov ct0 0%Z; Mov ct1 0%Z;
-    Mov cs0 0%Z; Mov cs1 0%Z; Jalr cnull cra;
-    Lea ca0 (-1)%Z; Store ca0 7%Z; Store ca1 9%Z; Jalr cnull cra
+    Store csp cra;
+    Lea csp 1%Z;
+    Mov ca0 csp;
+    GetA cs0 ca0;
+    machine_instructions.Add cs1 cs0 1%Z;
+    Subseg ca0 cs0 cs1;
+    Store ca0 0%Z;
+    Lea csp 1%Z;
+    Mov ctp PC;
+    GetB cs0 ctp;
+    GetA cs1 ctp;
+    Sub cs0 cs0 cs1;
+    Lea ctp cs0;
+    Mov ct0 ctp;
+    Lea ct0 0%Z;
+    Load ct0 ct0;
+    Mov ct1 ctp;
+    Lea ct1 1%Z;
+    Load ct1 ct1;
+    Mov ca1 ctp;
+    Lea ca1 2%Z;
+    Load ca1 ca1;
+    Mov cs0 0%Z;
+    Mov cs1 0%Z;
+    Mov cs0 cra;
+    Mov cs1 ct1;
+    Jalr cra ct0;
+    Lea csp (-1)%Z;
+    Lea csp (-1)%Z;
+    Load cra csp;
+    Mov ca0 0%Z;
+    Mov ca1 0%Z;
+    Mov ct0 0%Z;
+    Mov ct1 0%Z;
+    Mov cs0 0%Z;
+    Mov cs1 0%Z;
+    Jalr cnull cra;
+    Lea ca0 (-1)%Z;
+    Store ca0 7%Z;
+    Store ca1 9%Z;
+    Jalr cnull cra
   ].
 
 Definition so_C_data : list Word := [WInt 0].
@@ -107,10 +128,10 @@ Definition so_C_data : list Word := [WInt 0].
 Program Definition so_concrete_cmptSwitcher : cmptSwitcher.
 Proof.
   refine (@mkCmptSwitcher machine_parameters_instance
-    so_switcher_begin so_switcher_end so_switcher_call so_switcher_return
-    so_switcher_sealing_type so_trusted_stack_begin so_trusted_stack_end
+    so_switcher_b so_switcher_e so_switcher_call so_switcher_return
+    so_switcher_sealing_type so_trusted_stack_b so_trusted_stack_e
     _ _ _ _ (replicate 100 (WInt 0)) _ eq_refl
-    so_stack_begin so_stack_end (replicate 100 (WInt 0)) _ _).
+    so_stack_b so_stack_e (replicate 100 (WInt 0)) _ _).
   - vm_compute; solve_addr.
   - vm_compute; solve_addr.
   - vm_compute; solve_addr.
@@ -125,7 +146,7 @@ Defined.
 Program Definition so_concrete_cmptAssert : cmptAssert.
 Proof.
   refine (@mkCmptAssert machine_parameters_instance
-    so_assert_begin so_assert_end so_assert_cap so_assert_flag _ _ _ _).
+    so_assert_b so_assert_e so_assert_cap so_assert_flag _ _ _ _).
   - vm_compute; solve_addr.
   - vm_compute; solve_addr.
   - vm_compute; solve_addr.
@@ -140,16 +161,16 @@ Local Instance so_concrete_assertLayout : assertLayout.
 Proof. exact (cmptAssert_assertLayout so_concrete_cmptAssert). Defined.
 
 Definition so_C_f : Sealable :=
-  SCap RO Global so_C_exports_pcc so_C_exports_entries_end
-    so_C_exports_entries_begin.
+  SCap RO Global so_C_exports_pcc so_C_exports_entries_e
+    so_C_exports_entries_b.
 Definition so_C_g : Sealable :=
-  SCap RO Global so_C_exports_pcc so_C_exports_entries_end
-    (so_C_exports_entries_begin ^+ 1)%a.
+  SCap RO Global so_C_exports_pcc so_C_exports_entries_e
+    (so_C_exports_entries_b ^+ 1)%a.
 Definition so_main_imports_concrete : list Word := so_main_imports so_C_f.
 Definition so_C_imports : list Word :=
-  [ WSentry XSRW_ Local so_switcher_begin so_switcher_end so_switcher_call
+  [ WSentry XSRW_ Local so_switcher_b so_switcher_e so_switcher_call
   ; WSealed so_switcher_sealing_type
-      (so_entry_f_sb so_main_exports_pcc so_main_exports_entries_end)
+      (so_entry_f_sb so_main_exports_pcc so_main_exports_entries_e)
   ; WSealed so_switcher_sealing_type so_C_g
   ].
 Definition so_C_exports : list Word :=
@@ -157,9 +178,9 @@ Definition so_C_exports : list Word :=
 
 Program Definition so_concrete_main_cmpt : cmpt.
 Proof.
-  refine (@mkCmpt so_main_pcc_begin so_main_code_start so_main_pcc_end
-    so_main_data_begin so_main_data_end so_main_exports_pcc so_main_exports_cgp
-    so_main_exports_entries_begin so_main_exports_entries_end
+  refine (@mkCmpt so_main_pcc_b so_main_code_start so_main_pcc_e
+    so_main_data_b so_main_data_e so_main_exports_pcc so_main_exports_cgp
+    so_main_exports_entries_b so_main_exports_entries_e
     so_main_imports_concrete so_main_code so_main_data so_export_table_entries
     _ _ _ _ _ _ _).
   - vm_compute; solve_addr.
@@ -173,9 +194,9 @@ Defined.
 
 Program Definition so_concrete_C_cmpt : cmpt.
 Proof.
-  refine (@mkCmpt so_C_pcc_begin so_C_code_start so_C_pcc_end
-    so_C_data_begin so_C_data_end so_C_exports_pcc so_C_exports_cgp
-    so_C_exports_entries_begin so_C_exports_entries_end
+  refine (@mkCmpt so_C_pcc_b so_C_code_start so_C_pcc_e
+    so_C_data_b so_C_data_e so_C_exports_pcc so_C_exports_cgp
+    so_C_exports_entries_b so_C_exports_entries_e
     so_C_imports so_C_code so_C_data so_C_exports _ _ _ _ _ _ _).
   - vm_compute; solve_addr.
   - vm_compute; solve_addr.
@@ -218,13 +239,13 @@ Proof.
 Defined.
 
 Definition so_initial_registers : Reg :=
-  <[PC := WCap RX Global so_main_pcc_begin so_main_pcc_end so_main_code_start]>
-  (<[cgp := WCap RW Global so_main_data_begin so_main_data_end so_main_data_begin]>
-  (<[csp := WCap RWL Local so_stack_begin so_stack_end so_stack_begin]>
+  <[PC := WCap RX Global so_main_pcc_b so_main_pcc_e so_main_code_start]>
+  (<[cgp := WCap RW Global so_main_data_b so_main_data_e so_main_data_b]>
+  (<[csp := WCap RWL Local so_stack_b so_stack_e so_stack_b]>
     (gset_to_gmap (WInt 0) all_registers_s))).
 Definition so_initial_sregisters : SReg :=
-  <[MTDC := WCap RWL Local so_trusted_stack_begin so_trusted_stack_end
-      so_trusted_stack_begin]> ∅.
+  <[MTDC := WCap RWL Local so_trusted_stack_b so_trusted_stack_e
+      so_trusted_stack_b]> ∅.
 Definition so_initial_memory : Mem := mk_initial_memory.
 
 Lemma so_initial_registers_correct : is_initial_registers so_initial_registers.
@@ -258,7 +279,7 @@ Proof.
   - apply Forall_replicate; done.
 Qed.
 
-Theorem so_concrete_adequacy reg' sreg' mem' es :
+Lemma so_concrete_adequacy reg' sreg' mem' es :
   rtc erased_step
     ([Seq (Instr Executable)],
       (so_initial_registers, so_initial_sregisters, so_initial_memory))
