theories/case_studies/vae/vae_concrete.v
@@ -12,72 +12,65 @@ Local Notation "'A' z" :=
 Local Notation "'OT' z" :=
   (@finz.FinZ ONum z%Z eq_refl eq_refl) (at level 10).
 
-Definition vae_main_pcc_begin : Addr := A 9.
+Definition vae_main_pcc_b : Addr := A 9.
 Definition vae_main_code_start : Addr := A 12.
-Definition vae_main_pcc_end : Addr := A 84.
-Definition vae_C_pcc_begin : Addr := A 84.
+Definition vae_main_pcc_e : Addr := A 84.
+Definition vae_C_pcc_b : Addr := A 84.
 Definition vae_C_code_start : Addr := A 87.
-Definition vae_C_pcc_end : Addr := A 152.
-Definition vae_main_data_begin : Addr := A 152.
-Definition vae_main_data_end : Addr := A 153.
-Definition vae_C_data_begin : Addr := A 153.
-Definition vae_C_data_end : Addr := A 154.
+Definition vae_C_pcc_e : Addr := A 152.
+Definition vae_main_data_b : Addr := A 152.
+Definition vae_main_data_e : Addr := A 153.
+Definition vae_C_data_b : Addr := A 153.
+Definition vae_C_data_e : Addr := A 154.
 Definition vae_main_exports_pcc : Addr := A 154.
 Definition vae_main_exports_cgp : Addr := A 155.
-Definition vae_main_exports_entries_begin : Addr := A 156.
-Definition vae_main_exports_entries_end : Addr := A 157.
+Definition vae_main_exports_entries_b : Addr := A 156.
+Definition vae_main_exports_entries_e : Addr := A 157.
 Definition vae_C_exports_pcc : Addr := A 157.
 Definition vae_C_exports_cgp : Addr := A 158.
-Definition vae_C_exports_entries_begin : Addr := A 159.
-Definition vae_C_exports_entries_end : Addr := A 161.
-Definition vae_assert_begin : Addr := A 161.
+Definition vae_C_exports_entries_b : Addr := A 159.
+Definition vae_C_exports_entries_e : Addr := A 161.
+Definition vae_assert_b : Addr := A 161.
 Definition vae_assert_cap : Addr := A 173.
-Definition vae_assert_end : Addr := A 174.
+Definition vae_assert_e : Addr := A 174.
 Definition vae_assert_flag : Addr := A 174.
-Definition vae_switcher_begin : Addr := A 175.
+Definition vae_switcher_b : Addr := A 175.
 Definition vae_switcher_call : Addr := A 176.
 Definition vae_switcher_return : Addr := A 264.
-Definition vae_switcher_end : Addr := A 326.
+Definition vae_switcher_e : Addr := A 326.
 Definition vae_switcher_sealing_type : OType := OT 9.
-Definition vae_trusted_stack_begin : Addr := A 4096.
-Definition vae_trusted_stack_end : Addr := A 4196.
-Definition vae_stack_begin : Addr := A 1024.
-Definition vae_stack_end : Addr := A 1124.
+Definition vae_trusted_stack_b : Addr := A 4096.
+Definition vae_trusted_stack_e : Addr := A 4196.
+Definition vae_stack_b : Addr := A 1024.
+Definition vae_stack_e : Addr := A 1124.
 
 Ltac unfold_vae_addresses :=
-  unfold vae_main_pcc_begin, vae_main_code_start, vae_main_pcc_end,
-    vae_C_pcc_begin, vae_C_code_start, vae_C_pcc_end,
-    vae_main_data_begin, vae_main_data_end, vae_C_data_begin, vae_C_data_end,
+  unfold vae_main_pcc_b, vae_main_code_start, vae_main_pcc_e,
+    vae_C_pcc_b, vae_C_code_start, vae_C_pcc_e,
+    vae_main_data_b, vae_main_data_e, vae_C_data_b, vae_C_data_e,
     vae_main_exports_pcc, vae_main_exports_cgp,
-    vae_main_exports_entries_begin, vae_main_exports_entries_end,
+    vae_main_exports_entries_b, vae_main_exports_entries_e,
     vae_C_exports_pcc, vae_C_exports_cgp,
-    vae_C_exports_entries_begin, vae_C_exports_entries_end,
-    vae_assert_begin, vae_assert_cap, vae_assert_end, vae_assert_flag,
-    vae_switcher_begin, vae_switcher_call, vae_switcher_return,
-    vae_switcher_end, vae_switcher_sealing_type,
-    vae_trusted_stack_begin, vae_trusted_stack_end,
-    vae_stack_begin, vae_stack_end.
+    vae_C_exports_entries_b, vae_C_exports_entries_e,
+    vae_assert_b, vae_assert_cap, vae_assert_e, vae_assert_flag,
+    vae_switcher_b, vae_switcher_call, vae_switcher_return,
+    vae_switcher_e, vae_switcher_sealing_type,
+    vae_trusted_stack_b, vae_trusted_stack_e,
+    vae_stack_b, vae_stack_e.
 
 Ltac unfold_vae_addresses_in H :=
-  unfold vae_main_pcc_begin, vae_main_code_start, vae_main_pcc_end,
-    vae_C_pcc_begin, vae_C_code_start, vae_C_pcc_end,
-    vae_main_data_begin, vae_main_data_end, vae_C_data_begin, vae_C_data_end,
+  unfold vae_main_pcc_b, vae_main_code_start, vae_main_pcc_e,
+    vae_C_pcc_b, vae_C_code_start, vae_C_pcc_e,
+    vae_main_data_b, vae_main_data_e, vae_C_data_b, vae_C_data_e,
     vae_main_exports_pcc, vae_main_exports_cgp,
-    vae_main_exports_entries_begin, vae_main_exports_entries_end,
+    vae_main_exports_entries_b, vae_main_exports_entries_e,
     vae_C_exports_pcc, vae_C_exports_cgp,
-    vae_C_exports_entries_begin, vae_C_exports_entries_end,
-    vae_assert_begin, vae_assert_cap, vae_assert_end, vae_assert_flag,
-    vae_switcher_begin, vae_switcher_call, vae_switcher_return,
-    vae_switcher_end, vae_switcher_sealing_type,
-    vae_trusted_stack_begin, vae_trusted_stack_end,
-    vae_stack_begin, vae_stack_end in H.
-
-Definition vae_C_load (dst src : RegName) : instr.
-Proof.
-  constructor 5.
-  - exact dst.
-  - exact src.
-Defined.
+    vae_C_exports_entries_b, vae_C_exports_entries_e,
+    vae_assert_b, vae_assert_cap, vae_assert_e, vae_assert_flag,
+    vae_switcher_b, vae_switcher_call, vae_switcher_return,
+    vae_switcher_e, vae_switcher_sealing_type,
+    vae_trusted_stack_b, vae_trusted_stack_e,
+    vae_stack_b, vae_stack_e in H.
 
 (** The concrete adversary's first entry calls [awkward] with its second entry
     [g]. The callback [g] uses the adversary data cell as a one-shot flag: on
@@ -86,27 +79,72 @@ Defined.
     and restore their outer return capabilities around nested calls. *)
 Definition vae_C_code : list Word :=
   encodeInstrsW [
-    Store csp cra; Lea csp 1%Z;
-    Mov ct0 PC; GetB cs0 ct0; GetA cs1 ct0; Sub cs0 cs0 cs1;
-    Lea ct0 cs0; Lea ct0 0%Z; vae_C_load ct0 ct0; Mov cs0 0%Z;
-    Mov ct1 PC; GetB cs0 ct1; GetA cs1 ct1; Sub cs0 cs0 cs1;
-    Lea ct1 cs0; Lea ct1 1%Z; vae_C_load ct1 ct1; Mov cs0 0%Z;
-    Mov ca0 PC; GetB cs0 ca0; GetA cs1 ca0; Sub cs0 cs0 cs1;
-    Lea ca0 cs0; Lea ca0 2%Z; vae_C_load ca0 ca0; Mov cs0 0%Z;
+    Store csp cra;
+    Lea csp 1%Z;
+    Mov ct0 PC;
+    GetB cs0 ct0;
+    GetA cs1 ct0;
+    Sub cs0 cs0 cs1;
+    Lea ct0 cs0;
+    Lea ct0 0%Z;
+    Load ct0 ct0;
+    Mov cs0 0%Z;
+    Mov ct1 PC;
+    GetB cs0 ct1;
+    GetA cs1 ct1;
+    Sub cs0 cs0 cs1;
+    Lea ct1 cs0;
+    Lea ct1 1%Z;
+    Load ct1 ct1;
+    Mov cs0 0%Z;
+    Mov ca0 PC;
+    GetB cs0 ca0;
+    GetA cs1 ca0;
+    Sub cs0 cs0 cs1;
+    Lea ca0 cs0;
+    Lea ca0 2%Z;
+    Load ca0 ca0;
+    Mov cs0 0%Z;
     Jalr cra ct0;
-    Lea csp (-1)%Z; vae_C_load cra csp; Mov ca0 0%Z; Jalr cnull cra;
+    Lea csp (-1)%Z;
+    Load cra csp;
+    Mov ca0 0%Z;
+    Jalr cnull cra;
 
-    vae_C_load ct0 cgp; Jnz 31%Z ct0; Store cgp 1%Z;
-    Store csp cra; Lea csp 1%Z;
-    Mov ct0 PC; GetB cs0 ct0; GetA cs1 ct0; Sub cs0 cs0 cs1;
-    Lea ct0 cs0; Lea ct0 0%Z; vae_C_load ct0 ct0; Mov cs0 0%Z;
-    Mov ct1 PC; GetB cs0 ct1; GetA cs1 ct1; Sub cs0 cs0 cs1;
-    Lea ct1 cs0; Lea ct1 1%Z; vae_C_load ct1 ct1; Mov cs0 0%Z;
-    Mov ca0 PC; GetB cs0 ca0; GetA cs1 ca0; Sub cs0 cs0 cs1;
-    Lea ca0 cs0; Lea ca0 2%Z; vae_C_load ca0 ca0; Mov cs0 0%Z;
+    Load ct0 cgp;
+    Jnz 31%Z ct0;
+    Store cgp 1%Z;
+    Store csp cra;
+    Lea csp 1%Z;
+    Mov ct0 PC;
+    GetB cs0 ct0;
+    GetA cs1 ct0;
+    Sub cs0 cs0 cs1;
+    Lea ct0 cs0;
+    Lea ct0 0%Z;
+    Load ct0 ct0;
+    Mov cs0 0%Z;
+    Mov ct1 PC;
+    GetB cs0 ct1;
+    GetA cs1 ct1;
+    Sub cs0 cs0 cs1;
+    Lea ct1 cs0;
+    Lea ct1 1%Z;
+    Load ct1 ct1;
+    Mov cs0 0%Z;
+    Mov ca0 PC;
+    GetB cs0 ca0;
+    GetA cs1 ca0;
+    Sub cs0 cs0 cs1;
+    Lea ca0 cs0;
+    Lea ca0 2%Z;
+    Load ca0 ca0;
+    Mov cs0 0%Z;
     Jalr cra ct0;
-    Lea csp (-1)%Z; vae_C_load cra csp;
-    Mov ca0 0%Z; Jalr cnull cra
+    Lea csp (-1)%Z;
+    Load cra csp;
+    Mov ca0 0%Z;
+    Jalr cnull cra
   ].
 
 Definition vae_C_data : list Word := [WInt 0].
@@ -114,12 +152,12 @@ Definition vae_C_data : list Word := [WInt 0].
 Program Definition vae_concrete_cmptSwitcher : cmptSwitcher.
 Proof.
   refine (@mkCmptSwitcher machine_parameters_instance
-    vae_switcher_begin vae_switcher_end
+    vae_switcher_b vae_switcher_e
     vae_switcher_call vae_switcher_return vae_switcher_sealing_type
-    vae_trusted_stack_begin vae_trusted_stack_end
+    vae_trusted_stack_b vae_trusted_stack_e
     _ _ _ _
     (replicate 100 (WInt 0)) _ eq_refl
-    vae_stack_begin vae_stack_end (replicate 100 (WInt 0)) _ _).
+    vae_stack_b vae_stack_e (replicate 100 (WInt 0)) _ _).
   - vm_compute; solve_addr.
   - vm_compute; solve_addr.
   - vm_compute; solve_addr.
@@ -135,7 +173,7 @@ Defined.
 Program Definition vae_concrete_cmptAssert : cmptAssert.
 Proof.
   refine (@mkCmptAssert machine_parameters_instance
-    vae_assert_begin vae_assert_end vae_assert_cap vae_assert_flag _ _ _ _).
+    vae_assert_b vae_assert_e vae_assert_cap vae_assert_flag _ _ _ _).
   - vm_compute; solve_addr.
   - vm_compute; solve_addr.
   - vm_compute; solve_addr.
@@ -157,19 +195,19 @@ Proof.
 Defined.
 
 Definition vae_C_f : Sealable :=
-  SCap RO Global vae_C_exports_pcc vae_C_exports_entries_end
-    vae_C_exports_entries_begin.
+  SCap RO Global vae_C_exports_pcc vae_C_exports_entries_e
+    vae_C_exports_entries_b.
 
 Definition vae_C_g : Sealable :=
-  SCap RO Global vae_C_exports_pcc vae_C_exports_entries_end
-    (vae_C_exports_entries_begin ^+ 1)%a.
+  SCap RO Global vae_C_exports_pcc vae_C_exports_entries_e
+    (vae_C_exports_entries_b ^+ 1)%a.
 
 Definition vae_main_imports_concrete : list Word := vae_main_imports vae_C_f.
 
 Definition vae_C_imports : list Word :=
-  [ WSentry XSRW_ Local vae_switcher_begin vae_switcher_end vae_switcher_call
+  [ WSentry XSRW_ Local vae_switcher_b vae_switcher_e vae_switcher_call
   ; WSealed vae_switcher_sealing_type
-      (vae_entry_awkward_sb vae_main_exports_pcc vae_main_exports_entries_end)
+      (vae_entry_awkward_sb vae_main_exports_pcc vae_main_exports_entries_e)
   ; WSealed vae_switcher_sealing_type vae_C_g
   ].
 
@@ -179,10 +217,10 @@ Definition vae_C_exports : list Word :=
 Program Definition vae_concrete_main_cmpt : cmpt.
 Proof.
   refine (@mkCmpt
-    vae_main_pcc_begin vae_main_code_start vae_main_pcc_end
-    vae_main_data_begin vae_main_data_end
+    vae_main_pcc_b vae_main_code_start vae_main_pcc_e
+    vae_main_data_b vae_main_data_e
     vae_main_exports_pcc vae_main_exports_cgp
-    vae_main_exports_entries_begin vae_main_exports_entries_end
+    vae_main_exports_entries_b vae_main_exports_entries_e
     vae_main_imports_concrete vae_main_code vae_main_data vae_export_table_entries
     _ _ _ _ _ _ _).
   - vm_compute; solve_addr.
@@ -197,10 +235,10 @@ Defined.
 Program Definition vae_concrete_C_cmpt : cmpt.
 Proof.
   refine (@mkCmpt
-    vae_C_pcc_begin vae_C_code_start vae_C_pcc_end
-    vae_C_data_begin vae_C_data_end
+    vae_C_pcc_b vae_C_code_start vae_C_pcc_e
+    vae_C_data_b vae_C_data_e
     vae_C_exports_pcc vae_C_exports_cgp
-    vae_C_exports_entries_begin vae_C_exports_entries_end
+    vae_C_exports_entries_b vae_C_exports_entries_e
     vae_C_imports vae_C_code vae_C_data vae_C_exports
     _ _ _ _ _ _ _).
   - vm_compute; solve_addr.
@@ -244,15 +282,15 @@ Proof.
 Defined.
 
 Definition vae_initial_registers : Reg :=
-  <[PC := WCap RX Global vae_main_pcc_begin vae_main_pcc_end vae_main_code_start]>
-  (<[cgp := WCap RW Global vae_main_data_begin vae_main_data_end
-      vae_main_data_begin]>
-  (<[csp := WCap RWL Local vae_stack_begin vae_stack_end vae_stack_begin]>
+  <[PC := WCap RX Global vae_main_pcc_b vae_main_pcc_e vae_main_code_start]>
+  (<[cgp := WCap RW Global vae_main_data_b vae_main_data_e
+      vae_main_data_b]>
+  (<[csp := WCap RWL Local vae_stack_b vae_stack_e vae_stack_b]>
     (gset_to_gmap (WInt 0) all_registers_s))).
 
 Definition vae_initial_sregisters : SReg :=
-  <[MTDC := WCap RWL Local vae_trusted_stack_begin vae_trusted_stack_end
-      vae_trusted_stack_begin]> ∅.
+  <[MTDC := WCap RWL Local vae_trusted_stack_b vae_trusted_stack_e
+      vae_trusted_stack_b]> ∅.
 
 Definition vae_initial_memory : Mem := mk_initial_memory.
 
@@ -288,7 +326,7 @@ Proof.
   - apply Forall_replicate; done.
 Qed.
 
-Theorem vae_concrete_adequacy reg' sreg' mem' es :
+Lemma vae_concrete_adequacy reg' sreg' mem' es :
   rtc erased_step
     ([Seq (Instr Executable)],
       (vae_initial_registers, vae_initial_sregisters, vae_initial_memory))
